l4v-sabre: fix refine

spec/design/PSpaceFuns_H.thy
@@ -35,6 +35,7 @@ placeNewObject :: "machine_word \<Rightarrow> ('a :: pspace_storable) \<Rightarr
 consts
 placeNewObject' :: "machine_word \<Rightarrow> kernel_object \<Rightarrow> nat \<Rightarrow> unit kernel"
 
+
 consts
 deleteObjects :: "machine_word \<Rightarrow> nat \<Rightarrow> unit kernel"
 
@@ -128,6 +129,11 @@ defs placeNewObject'_def:
         modify (\<lambda> ks. ks \<lparr> ksPSpace := ps'\<rparr>)
 od)"
 
+definition deleteRange :: "( machine_word , 'a ) DataMap.map \<Rightarrow> machine_word \<Rightarrow> nat \<Rightarrow> ( machine_word , 'a ) DataMap.map"
+where "deleteRange m ptr bits \<equiv>
+        let inRange = (\<lambda>x. x && ((- mask bits) - 1) = fromPPtr ptr) in
+        data_map_filterWithKey (\<lambda> x _. Not (inRange x)) m"
+
 defs deleteObjects_def:
 "deleteObjects ptr bits\<equiv> (do
         unless (fromPPtr ptr && mask bits = 0) $
@@ -137,9 +143,7 @@ defs deleteObjects_def:
         doMachineOp $ freeMemory (PPtr (fromPPtr ptr)) bits;
         ps \<leftarrow> gets ksPSpace;
         inRange \<leftarrow> return ( (\<lambda> x. x && ((- mask bits) - 1) = fromPPtr ptr));
-        map' \<leftarrow> return ( data_map_filterWithKey
-                        (\<lambda> x _. Not (inRange x))
-                        (psMap ps));
+        map' \<leftarrow> return ( deleteRange (psMap ps) (fromPPtr ptr) bits);
         ps' \<leftarrow> return ( ps \<lparr> psMap := map' \<rparr>);
         modify (\<lambda> ks. ks \<lparr> ksPSpace := ps'\<rparr>);
         modify (\<lambda> ks. ks \<lparr> gsUserPages := (\<lambda> x. if inRange x
