proof/invariant-abstract/Machine_AI.thy
@@ -456,8 +456,7 @@ lemma no_irq_debugPrint: "no_irq (debugPrint $ xs)"
 
 
 lemma no_irq_ackInterrupt: "no_irq (ackInterrupt irq)"
-  by (clarsimp simp: no_irq_def ackInterrupt_def)
-
+  by (wp | clarsimp simp: no_irq_def ackInterrupt_def)+
 
 lemma no_irq_loadWord: "no_irq (loadWord x)"
   apply (clarsimp simp: no_irq_def)
