proof/invariant-abstract/VSpace_AI.thy
@@ -587,6 +587,8 @@ lemma invalidate_asid_entry_invs [wp]:
 
 lemmas cleanCaches_PoU_irq_masks = no_irq[OF no_irq_cleanCaches_PoU]
 
+lemmas ackInterrupt_irq_masks = no_irq[OF no_irq_ackInterrupt]
+
 lemma invalidate_I_PoU_underlying_memory[wp]:
   "\<lbrace>\<lambda>m'. underlying_memory m' p = um\<rbrace>
    invalidate_I_PoU
@@ -1715,6 +1717,16 @@ lemma dmo_setCurrentPD_invs[wp]: "\<lbrace>invs\<rbrace> do_machine_op (setCurre
      apply ((clarsimp simp: setCurrentPD_def writeTTBR0_def dsb_def isb_def machine_op_lift_def
                            machine_rest_lift_def split_def | wp)+)[3]
   apply(erule (1) use_valid[OF _ setCurrentPD_irq_masks])
+  done
+
+lemma dmo_ackInterrupt[wp]: "\<lbrace>invs\<rbrace> do_machine_op (ackInterrupt irq) \<lbrace>\<lambda>y. invs\<rbrace>"
+  apply (wp dmo_invs)
+  apply safe
+   apply (drule_tac Q="\<lambda>_ m'. underlying_memory m' p = underlying_memory m p"
+          in use_valid)
+     apply ((clarsimp simp: ackInterrupt_def machine_op_lift_def
+                           machine_rest_lift_def split_def | wp)+)[3]
+  apply(erule (1) use_valid[OF _ ackInterrupt_irq_masks])
   done
 
 lemma svr_invs [wp]:
@@ -3685,7 +3697,7 @@ lemma empty_table_pt_capI:
 
 crunch underlying_memory[wp]: cleanCacheRange_PoC, cleanL2Range, invalidateL2Range, invalidateByVA, 
                               cleanInvalidateL2Range, cleanInvalByVA, invalidateCacheRange_I, 
-                              branchFlushRange
+                              branchFlushRange, ackInterrupt
                            "\<lambda>m'. underlying_memory m' p = um"
   (wp: cacheRangeOp_lift simp: cache_machine_op_defs machine_op_lift_def machine_rest_lift_def split_def
    ignore: ignore_failure)
